spec/abstract/ARM/ArchVSpace_A.thy
@@ -325,7 +325,7 @@ definition
      | _ \<Rightarrow> throwError InvalidRoot) <catch>
     (\<lambda>_. do
        global_pd \<leftarrow> gets (arm_global_pd \<circ> arch_state);
-       do_machine_op $ set_current_pd $ addrFromPPtr global_pd
+       do_machine_op $ set_current_pd $ addrFromKPPtr global_pd
     od)
 od"
 
